make heavily allocated variables explicit as local program variables

src/0/Term.sml
@@ -707,8 +707,9 @@ fun strip_binder opt =
                                     end handle HOL_ERR _ => NONE)
  in fn tm =>
    let
+     open Unsynchronized
      val (prefixl,body) = peel f tm []
-     val AV = ref @{position} (Redblackmap.mkDict String.compare) : ((string,occtype)Redblackmap.dict) ref
+     val AV = ref (Redblackmap.mkDict String.compare) : ((string,occtype)Redblackmap.dict) ref
      fun peekInsert (key,data) =
         let open Redblackmap
         in case peek (!AV,key)
