src/HolSat/def_cnf.sml
@@ -60,10 +60,11 @@ val GCONJUNCTS  =
         fun findTF tm = total (HolKernel.find_term (fn t => is_T t orelse is_F t)) tm
         fun GCONJUNCTS'' th = GCONJUNCTS' th []
     in fn tm => fn th =>
-          let val ths0 = if is_neg tm andalso is_neg (rand tm)
+          let open Unsynchronized
+              val ths0 = if is_neg tm andalso is_neg (rand tm)
                          then CONJUNCTSR (CONV_RULE NOT_NOT_CONV th) else [th]
               val ths1 = List.map GCONJUNCTS'' ths0
-              val is_cnf = ref @{position} true
+              val is_cnf = ref true
               val ths2 =  List.map (fn th =>
                                        if is_clausal (concl th) then (true,th)
                                        else (is_cnf:=false;(false,th))) (List.concat ths1)
