src/real/Diff.sig
@@ -1,5 +1,5 @@
 signature Diff =
 sig
-   val basic_diffs :Thm.thm list ref @{position}
+   val basic_diffs :Thm.thm list ref
    val DIFF_CONV : Abbrev.conv
 end
