src/real/realLib.sig
@@ -14,7 +14,7 @@ sig
    (* Incorporates simpsets for bool, pair, and arithmetic *)
 
    (* Differentiation *)
-   val basic_diffs :thm list ref @{position}
+   val basic_diffs :thm list ref
    val DIFF_CONV : conv
 
 end
